@prefix dc: <http://purl.org/dc/elements/1.1/>.
@prefix foaf: <http://xmlns.com/foaf/0.1/>.
@prefix wot: <http://xmlns.com/wot/0.1/>.
@prefix rss: <http://purl.org/rss/1.0/>.
@prefix x: <http://tommorris.org/foaf#>.
@prefix rdfs: <http://www.w3.org/2000/01/rdf-schema#>.
@prefix xsd: <http://www.w3.org/2001/XMLSchema-datatypes#>.
@prefix owl: <http://www.w3.org/2002/07/owl#>.
@prefix : <http://tommorris.org/vocab/voperm/> .

:PermissibleThing a owl:Class;
  rdfs:label "Permissible thing"@en;
  rdfs:comment "A thing which permissions can be placed upon."@en.

# here we define a list of classes that can have permissions set on them.
foaf:PersonalProfileDocument rdfs:subClassOf :PermissibleThing .
sioc:Post rdfs:subClassOf :PermissibleThing .
foaf:Document rdfs:subClassOf :PermissibleThing .
rss:channel a rdfs:subClassOf :PermissibleThing .
rss:item a rdfs:subClassOf :PermissibleThing .
  # by inference, in non-RDF contexts, things which match the semantics of
  # RSS/Atom channel and item should be considered permissible things

:hasPermissionProfile owl:ObjectProperty;
  rdfs:label "has permission profile"@en;
  rdfs:domain :PermissibleThing;
  rdfs:range :PermissionProfile.

:PermissionProfile a owl:Class;
  rdfs:label "The profile showing what permissions are given for the resource."@en .

# Feature 1: Polling Frequency
#   User agents should know how often to poll a resource.
:pollFrequency a owl:DatatypeProperty;
  rdfs:label "Poll frequency"@en;
  rdfs:comment "The minimum amount of time that a user agent should allow between polling the resource again."@en;
  rdfs:domain :PermissionProfile;
  rdfs:range xsd:duration .

# TODO: property to describe requirements of use of if-modified-else and etags

# Feature 2: Syndication restrictions
#   User agents should know how to they are allowed to reuse a resource.
:allowsRepublication a owl:DatatypeProperty;
  rdfs:label "Allows republication"@en;
  rdfs:comment "Republication means that one is allowed to take the resource and republish it as a new resource. This is designed in such a way as to allow users to opt-out from 'splogs', even though this will be of perhaps minimal effectiveness"@en;
  rdfs:domain :PermissionProfile;
  rdfs:range xsd:boolean .

# TODO: build a private/public distinction

# Feature 3: Transmission of user information to commercial partners
# and sponsors
#   User agents should know whether or not content is to be reusable for 
#   sponsorship, advertising and other commercial repurposing.
:allowsCommercialSharing a owl:DatatypeProperty;
  rdfs:label "Allows commercial sharing"@en;
  rdfs:comment "If I were to publish some material on one site, I do not necessarily want it to be used for commercial purposes on other sites."@en;
  rdfs:domain :PermissionProfile;
  rdfs:range xsd:boolean.

:banned a owl:ObjectProperty;
  rdfs:label "Banned"@en;
  rdfs:comment "An agent or organization that has been banned from getting access to materials under this policy. This can be used for inference, such that a company could look at this property and see if it matches with their competitors to see whether or not permission to use the resource would likely be given."@en;
  rdfs:domain :PermissionProfile;
  rdfs:range foaf:Organization, foaf:Agent, foaf:Person.

:permitted a owl:ObjectProperty;
  rdfs:label "Permitted"@en;
  rdfs:comment "An agent or organization that has been explicitly permitted access to materials under this policy"@en;
  rdfs:domain :PermissionProfile;
  rdfs:range foaf:Organization, foaf:Agent, foaf:Person.
  
# author's note about banned/permitted:  http://tommorris.lighthouseapp.com/projects/15368-voperm/tickets/1-unsure-about-banned-permitted